Cleaning up binencoders library.

src/BinEncoders/Env/Examples/EthernetFrame.v
@@ -12,7 +12,7 @@ Require Import
         Fiat.QueryStructure.Specification.Representation.Tuple
         Fiat.BinEncoders.Env.BinLib.Core
         Fiat.BinEncoders.Env.Common.Specs
-        Fiat.BinEncoders.Env.Common.Compose
+        Fiat.BinEncoders.Env.Common.ComposeIf
         Fiat.BinEncoders.Env.Common.ComposeOpt
         Fiat.BinEncoders.Env.Automation.Solver
         Fiat.BinEncoders.Env.Lib2.FixListOpt
@@ -23,504 +23,394 @@ Require Import
         Fiat.BinEncoders.Env.Lib2.EnumOpt
         Fiat.BinEncoders.Env.Lib2.SumTypeOpt.
 
-Require Import
-        Bedrock.Word.
+Require Import Bedrock.Word.
 
 Import Vectors.VectorDef.VectorNotations.
 Open Scope string_scope.
 Open Scope Tuple_scope.
 
-Definition EthernetFrame :=
-  @Tuple <"Destination" :: Vector.t char 6,
-          "Source" :: Vector.t char 6,
-          "Type" :: BoundedString ["ARP"; "IP"; "RARP"],
-          "Data" :: list char>.
+Opaque pow2. (* Don't want to be evaluating this. *)
+Opaque natToWord. (* Or this. *)
 
-Definition EtherTypeCodes : Vector.t (word 16) 3 :=
-  [WO~0~0~0~0~0~0~0~0~0~0~0~1~0~0~0~0;
-   WO~0~1~1~0~0~0~0~0~0~0~0~1~0~0~0~0;
-   WO~1~0~1~0~1~1~0~0~0~0~0~1~0~0~0~0
-  ].
+Ltac apply_compose :=
+  intros;
+  match goal with
+    H : cache_inv_Property ?P ?P_inv |- _ =>
+    first [eapply (compose_encode_correct_no_dep H); clear H
+          | eapply (compose_encode_correct H); clear H
+          | eapply (composeIf_encode_correct H); clear H
+          ]
+  end.
 
-  Definition transformer : Transformer ByteString := ByteStringTransformer.
+Ltac makeEvar T k :=
+  let x := fresh in evar (x : T); let y := eval unfold x in x in clear x; k y.
 
-  Local Notation "x ++ y" := (transform x y).
+Ltac shelve_inv :=
+  let H' := fresh in
+  let data := fresh in
+  intros data H';
+  repeat destruct H';
+  match goal with
+  | H : ?P data |- ?P_inv' =>
+    is_evar P;
+    let P_inv' := (eval pattern data in P_inv') in
+    let P_inv := match P_inv' with ?P_inv data => P_inv end in
+    let new_P_T := type of P in
+    makeEvar new_P_T
+             ltac:(fun new_P =>
+                     unify P (fun data => new_P data /\ P_inv data)); apply (Logic.proj2 H)
+  end.
 
-Definition composeIf E B
-           (transformer : Transformer B)
-           (encode1 : E -> Comp (B * E))
-           (iComp : Comp bool)
-           (encodeT : E -> Comp (B * E))
-           (encodeE : E -> Comp (B * E))
-  :=
-  (fun e0 =>
-     `(p, e1) <- encode1 e0;
-       b <- iComp;
-       If b Then
-          `(q, e2) <- encodeT e1;
-          ret (transform p q, e2)
-       Else (`(q, e2) <- encodeE e1;
-            ret (transform p q, e2))
-  )%comp.
+Definition transformer : Transformer ByteString := ByteStringTransformer.
 
-Lemma composeIf_encode_correct
-      {A A' B}
-      {cache : Cache}
-      {P  : CacheDecode -> Prop}
-      {P_inv1 P_invT P_invE : (CacheDecode -> Prop) -> Prop}
-      (P_inv_pf : cache_inv_Property P (fun P => P_inv1 P /\ P_invT P /\ P_invE P))
-      (transformer : Transformer B)
-      (project : A -> A')
-      (predicate : A -> Prop)
-      (predicate_rest : A' -> B -> Prop)
-      (predicate_rest' : A -> B -> Prop)
-      (predicate' : A' -> Prop)
-      (encode1 : A' -> CacheEncode -> Comp (B * CacheEncode))
-      (decode1 : B -> CacheDecode -> option (A' * B * CacheDecode))
-      (IComp : Comp bool)
-      (ICompb : A' -> B -> CacheDecode -> bool)
-      (encodeT : A -> CacheEncode -> Comp (B * CacheEncode))
-      (decodeT : A' -> B -> CacheDecode -> option (A * B * CacheDecode))
-      (encodeE : A -> CacheEncode -> Comp (B * CacheEncode))
-      (decodeE : A' -> B -> CacheDecode -> option (A * B * CacheDecode))
-      (decode1_pf :
-         cache_inv_Property P P_inv1
-         -> encode_decode_correct_f
-              cache transformer predicate' predicate_rest
-              encode1 decode1 P)
-      (decodeT_pf : forall proj,
-          computes_to IComp true ->
-          predicate' proj ->
-          cache_inv_Property P P_invT ->
-          encode_decode_correct_f
-            cache transformer
-            (fun data => predicate data /\ project data = proj)
-            predicate_rest'
-            encodeT
-            (decodeT proj) P)
-      (decodeE_pf : forall proj,
-          computes_to IComp false ->
-          predicate' proj ->
-          cache_inv_Property P P_invE ->
-          encode_decode_correct_f
-            cache transformer
-            (fun data => predicate data /\ project data = proj)
-            predicate_rest'
-            encodeE
-            (decodeE proj) P)
-      (ICompb_decT :
-         forall data env b b' c xenv c' ext,
-           predicate data
-           -> encode1 (project data) env ↝ (b, c)
-           -> IComp ↝ true
-           -> encodeT data c ↝ (b', xenv)
-           -> Equiv c c'
-           -> ICompb (project data) (transform b' ext) c' = true)
-      (ICompb_decE :
-         forall data env b b' c xenv c' ext,
-           predicate data
-           -> encode1 (project data) env ↝ (b, c)
-           -> IComp ↝ false
-           -> encodeE data c ↝ (b', xenv)
-           -> Equiv c c'
-           -> ICompb (project data) (transform b' ext) c' = false)
-      (ICompb_dec :
-         forall a b cd,
-           computes_to IComp (ICompb a b cd))
-      (predicate_rest_implT : forall a' b b'',
-          (IComp true /\
-          exists a ce ce' ce'' b' b'',
-            computes_to (encode1 a' ce) (b', ce')
-            /\ project a = a'
-            /\ predicate a
-            /\ computes_to (encodeT a ce') (b'', ce'')
-            /\ predicate_rest' a b)
-          -> predicate_rest a' (transform b'' b))
-      (predicate_rest_implE : forall a' b b'',
-          (IComp false /\
-          exists a ce ce' ce'' b',
-            computes_to (encode1 a' ce) (b', ce')
-            /\ project a = a'
-            /\ predicate a
-            /\ computes_to (encodeE a ce') (b'', ce'')
-            /\ predicate_rest' a b)
-          -> predicate_rest a' (transform b'' b))
-      (pred_pf : forall data, predicate data -> predicate' (project data))
+Theorem decode_list_all_correct_ComposeOpt
   : encode_decode_correct_f
-      cache transformer
-      (fun a => predicate a)
-      predicate_rest'
-      (fun (data : A) (ctx : CacheEncode) =>
-         composeIf _ _ _ (encode1 (project data)) IComp (encodeT data) (encodeE data)  ctx
-      )%comp
-     (fun (bin : B) (env : CacheDecode) =>
-        `(proj, rest, env') <- decode1 bin env;
-          If ICompb proj rest env' Then
-             decodeT proj rest env'
-             Else
-             decodeE proj rest env'
-     ) P.
+      _ transformer
+      (fun a => True)
+      (fun _ b => b = transform_id)
+      (encode_list_Spec encode_word_Spec)
+      (fun (bin : ByteString) (env : CacheDecode) =>
+         Some (byteString bin, ByteString_id, tt))
+      (fun a => True).
 Proof.
-  unfold cache_inv_Property in *; split.
-  { intros env env' xenv data bin ext env_pm pred_pm pred_pm_rest com_pf.
-    unfold composeIf, Bind2 in com_pf; computes_to_inv; destruct v;
-      destruct v0; simpl in com_pf''.
-    - computes_to_inv; destruct v; subst.
-      destruct (fun H => proj1 (decode1_pf (proj1 P_inv_pf)) _ _ _ _ _ (transform b0 ext) env_pm (pred_pf _ pred_pm) H com_pf); intuition; simpl in *; injections.
-      eapply predicate_rest_implT; repeat eexists; intuition eauto.
-      destruct (fun H' => proj1 (decodeT_pf (project data) com_pf' (pred_pf _ pred_pm)
-                                  H)
-                      _ _ _ _ _ ext H3 (conj pred_pm (eq_refl _)) H' com_pf'');
-        intuition; simpl in *; injections.
-      pose proof (ICompb_decT _ _ _ _ _ _ _ ext pred_pm com_pf com_pf' com_pf'' H3).
-      setoid_rewrite <- transform_assoc; rewrite H2.
-      intuition; simpl in *; injections.
-      rewrite H5, H6; simpl; eauto.
-    - computes_to_inv; destruct v; subst.
-      destruct (fun H' => proj1 (decode1_pf (proj1 P_inv_pf)) _ _ _ _ _ (transform b0 ext) env_pm (pred_pf _ pred_pm) H' com_pf); intuition; simpl in *; injections.
-      eapply predicate_rest_implE; intuition; repeat eexists; intuition eauto.
-      pose proof (ICompb_decE _ _ _ _ _ _ _ ext pred_pm com_pf com_pf' com_pf'' H3).
-      destruct (fun H' => proj1 (decodeE_pf (project data) com_pf' (pred_pf _ pred_pm)
-                                  H4)
-                      _ _ _ _ _ ext H3 (conj pred_pm (eq_refl _)) H' com_pf'');
-        intuition; simpl in *; injections.
-      setoid_rewrite <- transform_assoc; rewrite H2.
-      intuition; simpl in *; injections.
-      rewrite H5, H7; simpl; eauto.
+  split.
+  {
+    intros env env' xenv l l' ext Eeq Ppred Ppred_rest Penc.
+    intuition; subst.
+    generalize dependent env. generalize dependent env'.
+    generalize dependent xenv.
+    generalize dependent l'. induction l.
+    { intros.
+      simpl in *; intuition; computes_to_inv;
+        injections; simpl.
+      eexists; eauto. }
+    { intros; simpl in *.
+      unfold Bind2 in Penc; computes_to_inv; subst.
+      destruct v; destruct v0; simpl in *.
+      injections.
+      eapply IHl in Penc'; eauto.
+      destruct_ex; intuition; injections.
+      pose proof transform_assoc;
+        pose proof transform_id_right.
+      simpl in H, H0.
+      setoid_rewrite <- H.
+      setoid_rewrite H0; eexists; intuition; repeat f_equal.
+      unfold encode_word_Spec in Penc.
+      simpl in Penc.
+      admit.
+    }
   }
-  { intros.
-    destruct (decode1 bin env') as [ [ [? ?] ? ] | ] eqn : ? ;
-      simpl in *; try discriminate.
-    pose proof (ICompb_dec a b c) as ICompb'.
-    destruct (ICompb a b c) eqn: ?; simpl in *.
-    - eapply (proj2 (decode1_pf (proj1 P_inv_pf))) in Heqo; eauto;
-        destruct Heqo; destruct_ex; intuition;
-          eapply (proj2 (decodeT_pf a ICompb' H7 H3)) in H1; eauto;
-            destruct H1; destruct_ex; intuition; subst.
-      eexists; eexists; repeat split.
-      repeat computes_to_econstructor; eauto.
-      simpl; repeat computes_to_econstructor; eauto.
-      simpl; rewrite transform_assoc; reflexivity.
-      eassumption.
-      eassumption.
-    - eapply (proj2 (decode1_pf (proj1 P_inv_pf))) in Heqo; eauto;
-        destruct Heqo; destruct_ex; intuition;
-          eapply (proj2 (decodeE_pf a ICompb' H7 H8)) in H1; eauto;
-            destruct H1; destruct_ex; intuition; subst.
-      eexists; eexists; repeat split.
-      repeat computes_to_econstructor; eauto.
-      simpl; repeat computes_to_econstructor; eauto.
-      simpl; rewrite transform_assoc; reflexivity.
-      eassumption.
-      eassumption.
+  { admit.
   }
 Qed.
 
-Local Notation "x 'ThenIf' i 'TheniC' t 'ElseiC' e " :=
-  (composeIf _ _ _ x i t e) (at level 100, right associativity).
+Ltac solve_data_inv :=
+  first [ simpl; intros; exact I
+        | shelve_inv ].
 
-  Definition encode_EthernetFrame_Spec (eth : EthernetFrame) :=
-      (encode_Vector_Spec encode_word_Spec eth!"Destination")
-        ThenC (encode_Vector_Spec encode_word_Spec eth!"Source")
-        ThenIf ({v1042 : bool | True}) (* Support both kinds of frames.*)
-        TheniC
-        (encode_nat_Spec 16 (length eth!"Data")
-           ThenC encode_word_Spec (WO~0~1~0~1~0~1~0~1)
-           ThenC encode_word_Spec (WO~0~1~0~1~0~1~0~1)
-           ThenC encode_word_Spec (WO~1~1~0~0~0~0~0~0)
-           ThenC encode_word_Spec (wzero 24)
-           ThenC encode_enum_Spec EtherTypeCodes eth!"Type"
-           ThenC encode_list_Spec encode_word_Spec eth!"Data"
-           DoneC)
-       ElseiC
-       encode_enum_Spec EtherTypeCodes eth!"Type"
-       ThenC encode_list_Spec encode_word_Spec eth!"Data"
-       DoneC.
-
-  Opaque pow2. (* Don't want to be evaluating this. *)
-
-  Ltac apply_compose :=
-    intros;
-    match goal with
-      H : cache_inv_Property ?P ?P_inv |- _ =>
-      first [eapply (compose_encode_correct_no_dep H); clear H
-            | eapply (compose_encode_correct H); clear H
-            | eapply (composeIf_encode_correct H); clear H
-            ]
-    end.
-
-  Ltac makeEvar T k :=
-    let x := fresh in evar (x : T); let y := eval unfold x in x in clear x; k y.
-
-  Ltac shelve_inv :=
-    let H' := fresh in
-    let data := fresh in
-    intros data H';
-    repeat destruct H';
-    match goal with
-    | H : ?P data |- ?P_inv' =>
-      is_evar P;
-      let P_inv' := (eval pattern data in P_inv') in
-      let P_inv := match P_inv' with ?P_inv data => P_inv end in
-      let new_P_T := type of P in
-      makeEvar new_P_T
-               ltac:(fun new_P =>
-                       unify P (fun data => new_P data /\ P_inv data)); apply (Logic.proj2 H)
-    end.
-
-  Theorem decode_list_all_correct_ComposeOpt
-      : encode_decode_correct_f
-          _ transformer
-          (fun a => True)
-          (fun _ b => b = transform_id)
-          (encode_list_Spec encode_word_Spec)
-          (fun (bin : ByteString) (env : CacheDecode) =>
-             Some (byteString bin, ByteString_id, tt))
-          (fun a => True).
-  Proof.
-    split.
-    {
-      intros env env' xenv l l' ext Eeq Ppred Ppred_rest Penc.
-      intuition; subst.
-      generalize dependent env. generalize dependent env'.
-      generalize dependent xenv.
-      generalize dependent l'. induction l.
-      { intros.
-        simpl in *; intuition; computes_to_inv;
-          injections; simpl.
-        eexists; eauto. }
-      { intros; simpl in *.
-        unfold Bind2 in Penc; computes_to_inv; subst.
-        destruct v; destruct v0; simpl in *.
-        injections.
-        eapply IHl in Penc'; eauto.
-        destruct_ex; intuition; injections.
-        pose proof transform_assoc;
-          pose proof transform_id_right.
-        simpl in H, H0.
-        setoid_rewrite <- H.
-        setoid_rewrite H0; eexists; intuition; repeat f_equal.
-        unfold encode_word_Spec in Penc.
-        simpl in Penc.
-        admit.
-      }
-    }
-    { admit.
-    }
-  Qed.
-
-  Ltac solve_data_inv :=
-    first [ simpl; intros; exact I
-          | shelve_inv ].
-
-  Lemma Vector_predicate_rest_True n
-    : forall a' b,
-      Vector_predicate_rest (fun (_ : word 8) (_ : ByteString) => True) encode_word_Spec n a' b.
-  Proof.
-    induction a'; simpl; eauto.
-  Qed.
-
-  Ltac finalize_decoder P_inv :=
+Ltac finalize_decoder P_inv :=
   (unfold encode_decode_correct_f; intuition eauto);
-    [ computes_to_inv; injections; subst; simpl;
+  [ computes_to_inv; injections; subst; simpl;
+    match goal with
+      H : Equiv _ ?env |- _ =>
+      eexists env; intuition eauto;
+      simpl;
       match goal with
-        H : Equiv _ ?env |- _ =>
-        eexists env; intuition eauto;
-        simpl;
-        match goal with
-          |- ?f ?a ?b ?c = ?P =>
-          let P' := (eval pattern a, b, c in P) in
-          let f' := match P' with ?f a b c => f end in
-          unify f f'; reflexivity
+        |- ?f ?a ?b ?c = ?P =>
+        let P' := (eval pattern a, b, c in P) in
+        let f' := match P' with ?f a b c => f end in
+        unify f f'; reflexivity
+      end
+    end
+  | injections; eauto
+  | eexists _; eexists _;
+    intuition eauto; injections; eauto using idx_ibound_eq;
+    try match goal with
+          |- P_inv ?data => destruct data;
+                            simpl in *; eauto
         end
-      end
-    | injections; eauto
-    | eexists _; eexists _;
-      intuition eauto; injections; eauto using idx_ibound_eq;
-      try match goal with
-        |- P_inv ?data => destruct data;
-                                 simpl in *; eauto
-      end
-    ].
+  ].
 
-  Lemma Check_Integrity {A B C D E F}
-        (b_eq_dec : forall b', DecideableEnsembles.DecideableEnsemble (fun b : B => b = b'))
-    : forall (a a' : A) (f : A -> B) (b : B) (f' : A -> C -> D -> option F) f'' (c : C) (d : D) (e : E) (P : E -> E -> Prop),
-      a = a'
-      -> f a = b
-      -> (exists e' : E,
-          f' a' c d = Some (f'' e') /\ P e e')
-      -> exists e' : E,
-          If DecideableEnsembles.dec (DecideableEnsemble := b_eq_dec b) (f a') Then f' a' c d Else None = Some (f'' e') /\ P e e'.
-  Proof.
-    intros.
-    rewrite H in H0.
-    intros; apply (DecideableEnsembles.dec_decides_P (DecideableEnsemble := b_eq_dec b)) in H0.
-    rewrite H0; simpl; intros; eauto.
-  Qed.
+(* Start Example Derivation. *)
 
-  Definition ethernet_Frame_OK (e : EthernetFrame) := lt (|e!"Data"|) 1501.
+Definition EthernetFrame :=
+  @Tuple <"Destination" :: Vector.t char 6,
+  "Source" :: Vector.t char 6,
+  "Type" :: BoundedString ["ARP"; "IP"; "RARP"],
+  "Data" :: list char>.
 
-  Lemma ethernet_Frame_OK_good_Len
-    : forall (e : EthernetFrame),
-      ethernet_Frame_OK e
-      -> lt (|e!"Data"|) (pow2 16).
-  Proof.
-    unfold ethernet_Frame_OK; intro.
-    match goal with |- context [| ?e |] => remember (|e|) end.
-    clear Heqn e.
-    etransitivity; eauto.
-    rewrite <- (wordToNat_natToWord_idempotent 16 1501).
-    eapply wordToNat_bound.
-    simpl; eapply BinNat.N.ltb_lt; reflexivity.
-  Qed.
+Definition EtherTypeCodes : Vector.t (word 16) 3 :=
+  [WO~0~0~0~0~1~0~0~0~0~0~0~0~0~0~0~0;
+   WO~0~0~0~0~1~0~0~0~0~0~0~0~0~1~1~0;
+   WO~0~0~0~0~1~0~0~0~0~0~1~1~0~1~0~1
+  ].
 
-  Global Instance Query_eq_nat : DecideableEnsembles.Query_eq nat :=
-    {| A_eq_dec := Coq.Arith.Peano_dec.eq_nat_dec |}.
+Definition encode_EthernetFrame_Spec (eth : EthernetFrame) :=
+  (encode_Vector_Spec encode_word_Spec eth!"Destination")
+    ThenC (encode_Vector_Spec encode_word_Spec eth!"Source")
+    ThenC Either
+    encode_nat_Spec 16 (|eth!"Data"|)
+    ThenC encode_word_Spec (WO~0~1~0~1~0~1~0~1)
+    ThenC encode_word_Spec (WO~0~1~0~1~0~1~0~1)
+    ThenC encode_word_Spec (WO~1~1~0~0~0~0~0~0)
+    ThenC encode_word_Spec (wzero 24)
+    ThenC encode_enum_Spec EtherTypeCodes eth!"Type"
+    ThenC encode_list_Spec encode_word_Spec eth!"Data"
+    DoneC
+    Or encode_enum_Spec EtherTypeCodes eth!"Type"
+    ThenC encode_list_Spec encode_word_Spec eth!"Data"
+    DoneC.
 
-  Definition packet_decoder
-    : { decodePlusCacheInv |
-        exists P_inv,
-        (cache_inv_Property (snd decodePlusCacheInv) P_inv
-        -> encode_decode_correct_f _ transformer ethernet_Frame_OK (fun _ b => b = ByteString_id) encode_EthernetFrame_Spec (fst decodePlusCacheInv) (snd decodePlusCacheInv))
-        /\ cache_inv_Property (snd decodePlusCacheInv) P_inv}.
-  Proof.
-    eexists (_, _); eexists _; split; simpl.
-    intros.
-    apply_compose.
-    intro. eapply Vector_decode_correct.
-    revert H; eapply Word_decode_correct.
-    solve_data_inv.
-    intros; apply Vector_predicate_rest_True.
-    intros;
+Definition ethernet_Frame_OK (e : EthernetFrame) := lt (|e!"Data"|) 1501.
+
+Lemma ethernet_Frame_OK_good_Len
+  : forall (e : EthernetFrame),
+    ethernet_Frame_OK e
+    -> lt (|e!"Data"|) (pow2 16).
+Proof.
+  unfold ethernet_Frame_OK; intro.
+  match goal with |- context [| ?e |] => remember (|e|) end.
+  clear Heqn e.
+  etransitivity; eauto.
+  rewrite <- (wordToNat_natToWord_idempotent 16 1501).
+  eapply wordToNat_bound.
+  simpl; eapply BinNat.N.ltb_lt; reflexivity.
+Qed.
+
+Definition v1042_test (b : ByteString) : bool :=
+  match byteString_get_word _ _ 16 b with
+  | Some w => if wlt_dec w (natToWord 16 1501) then true else false
+  | _ => false
+  end.
+
+Lemma v1042_OKT
+  : forall (data : EthernetFrame) (bin : ByteString) (env xenv : CacheEncode) (ext : ByteString),
+   ethernet_Frame_OK data ->
+   (encode_nat_Spec 16 (|data!"Data" |)
+    ThenC encode_word_Spec WO~0~1~0~1~0~1~0~1
+          ThenC encode_word_Spec WO~0~1~0~1~0~1~0~1
+                ThenC encode_word_Spec WO~1~1~0~0~0~0~0~0
+                      ThenC encode_word_Spec (wzero 24) ThenC encode_enum_Spec EtherTypeCodes data!"Type" ThenC encode_list_Spec encode_word_Spec data!"Data" DoneC) env
+   ↝ (bin, xenv) -> v1042_test (transform bin ext) = true.
+Proof.
+  unfold ethernet_Frame_OK; intros.
+  unfold compose at 1 in H0; unfold Bind2 in H0;
+    computes_to_inv; destruct v; destruct v0; simpl in *;
+        injections.
+  unfold encode_nat_Spec, encode_word_Spec in H0; computes_to_inv.
+  pose proof (f_equal fst H0) as H'; simpl in H'; rewrite <- H'.
+  pose proof transform_assoc as H''; simpl in H''; rewrite <- H''.
+  unfold v1042_test.
+  rewrite byteString_get_encode_word'; find_if_inside; eauto.
+  destruct n.
+  eapply natToWord_wlt; eauto; try reflexivity.
+  etransitivity.
+  unfold BinNat.N.lt; rewrite <- Nnat.Nat2N.inj_compare.
+  eapply Compare_dec.nat_compare_lt; eassumption.
+  reflexivity.
+Qed.
+
+Lemma VectorIn_cons {A} {n}
+  : forall (v : Vector.t A n) a a',
+    Vector.In a' (a :: v) -> a = a' \/ Vector.In a' v.
+Proof.
+  intros; inversion H; subst; eauto.
+  apply Eqdep_dec.inj_pair2_eq_dec in H3; subst; eauto using Peano_dec.eq_nat_dec.
+Qed.
+
+Lemma forall_Vector_P {A} (P : A -> Prop) {n}
+  : forall v : Vector.t A n,
+    Vector.Forall P v
+    -> forall idx, P (v[@idx]).
+Proof.
+  induction v; simpl; intros.
+  - inversion idx.
+  - revert v IHv H; pattern n, idx; apply Fin.caseS; simpl;
+      intros; inversion H; subst; eauto.
+    eapply IHv.
+    apply Eqdep_dec.inj_pair2_eq_dec in H2; subst; eauto using Peano_dec.eq_nat_dec.
+Qed.
+
+Ltac Discharge_NoDupVector :=
+  match goal with
+  |- NoDupVector _ =>
+  repeat econstructor; intro;
+  repeat match goal with
+         | H : Vector.In _ _ |- _ =>
+           first [apply VectorIn_cons in H; destruct H; try discriminate
+                 | inversion H]
+         end
+  end.
+
+Lemma v1042_OKE
+  : forall (data : EthernetFrame) (bin : ByteString) (env xenv : CacheEncode) (ext : ByteString),
+    ethernet_Frame_OK data
+    -> (encode_enum_Spec EtherTypeCodes data!"Type" ThenC encode_list_Spec encode_word_Spec data!"Data" DoneC) env ↝ (bin, xenv)
+    -> v1042_test (transform bin ext) = false.
+Proof.
+  unfold ethernet_Frame_OK; intros.
+  unfold compose at 1 in H0; unfold Bind2 in H0;
+    computes_to_inv; destruct v; destruct v0; simpl in *;
+        injections.
+  unfold encode_enum_Spec, encode_word_Spec in H0; computes_to_inv.
+  pose proof (f_equal fst H0) as H'; unfold fst in H'; rewrite <- H'.
+  pose proof transform_assoc as H''; simpl in H''; rewrite <- H''.
+  unfold v1042_test.
+  rewrite byteString_get_encode_word'; find_if_inside; eauto.
+  revert w; clear.
+  match goal with
+    |- context [Vector.nth (m := ?n) ?w ?idx] => remember idx; clear
+  end.
+  Local Transparent natToWord.
+  eapply forall_Vector_P; repeat econstructor;
+    unfold wlt; compute; intros; discriminate.
+Qed.
+
+Definition EthernetFrame_decoder
+  : { decodePlusCacheInv |
+      exists P_inv,
+      (cache_inv_Property (snd decodePlusCacheInv) P_inv
+       -> encode_decode_correct_f _ transformer ethernet_Frame_OK (fun _ b => b = ByteString_id) encode_EthernetFrame_Spec (fst decodePlusCacheInv) (snd decodePlusCacheInv))
+      /\ cache_inv_Property (snd decodePlusCacheInv) P_inv}.
+Proof.
+  eexists (_, _); eexists _; split; simpl.
+  intros.
+  apply_compose.
+  intro. eapply Vector_decode_correct.
+  revert H; eapply Word_decode_correct.
+  solve_data_inv.
+  intros; apply Vector_predicate_rest_True.
+  apply_compose.
+  intro. eapply Vector_decode_correct.
+  revert H0; eapply Word_decode_correct.
+  solve_data_inv.
+  intros; apply Vector_predicate_rest_True.
+  intros;
     match goal with
       H : cache_inv_Property ?P ?P_inv |- _ =>
-      eapply (composeIf_encode_correct H) with
-      (ICompb := fun _ b cd => match decode_nat (pow2 16 - 1) 16 b cd with
-                               | Some (b', _, _) => if Compare_dec.lt_dec 1500 b' then true else false
-                               | None => false end); clear H
+      eapply (composeIf'_encode_correct H)
+      with (ICompb := v1042_test)
     end.
-    intro; eapply Vector_decode_correct.
-    revert H0; eapply Word_decode_correct.
-    apply_compose.
-    eapply Nat_decode_correct with (sz' := 1500).
-    rewrite <- (wordToNat_natToWord_idempotent 16 1500).
-    eapply wordToNat_bound.
-    simpl; eapply BinNat.N.ltb_lt; reflexivity.
-    intuition.
-    simpl; intros; exact I.
-    apply_compose.
-    eapply Word_decode_correct.
-    solve_data_inv.
-    simpl; intros; exact I.
-    apply_compose.
-    eapply Word_decode_correct.
-    solve_data_inv.
-    simpl; intros; exact I.
-    apply_compose.
-    eapply Word_decode_correct.
-    solve_data_inv.
-    simpl; intros; exact I.
-    apply_compose.
-    eapply Word_decode_correct.
-    solve_data_inv.
-    simpl; intros; exact I.
-    apply_compose.
-    eapply Enum_decode_correct.
-    admit.
-    solve_data_inv.
-    simpl; intros; exact I.
-    apply_compose.
-    intros; eapply decode_list_all_correct_ComposeOpt.
-    solve_data_inv.
-    simpl; intros.
-    computes_to_inv; injections.
-    pose proof transform_id_left as H'; simpl in H'; rewrite H'; reflexivity.
-    simpl; intros.
-    unfold encode_decode_correct_f; intuition eauto.
-    match goal with
-      [H : ?p = ?proj1, H2 : ?f ?p = ?proj2 |-
-       exists xenv', ?f' ?proj1 ?b ?env' = Some (?data, ?ext, xenv') /\ Equiv xenv xenv'] =>
-      instantiate (1 := fun p b' c => if (DecideableEnsembles.A_eq_dec (f p) proj2) then _ p b' c else None); cbv beta
-    end.
-    destruct (@DecideableEnsembles.A_eq_dec nat Query_eq_nat
-               (@Datatypes.length char proj3) proj1); try congruence.
-    destruct data as [? [? [? [? [ ] ] ] ] ];
-      unfold GetAttribute, GetAttributeRaw in *;
-      simpl in *.
-    computes_to_inv; injections; subst; simpl.
-    pose proof transform_id_left as H'; simpl in H'; rewrite H'.
-    eexists env'; simpl; intuition eauto.
-    match goal with
-      |- ?f ?a ?b ?c = ?P =>
-      let P' := (eval pattern a, b, c in P) in
-      let f' := match P' with ?f a b c => f end in
-      try unify f f'; try reflexivity
-    end.
-    cbv beta in H12.
-    destruct (@DecideableEnsembles.A_eq_dec nat Query_eq_nat
-                                              (@Datatypes.length char proj3) proj1); try congruence; subst.
-    eexists _; eexists tt;
-      intuition eauto; injections; eauto using idx_ibound_eq;
-        try match goal with
-              |-  ?data => destruct data;
-                             simpl in *; eauto
-            end.
-    destruct env; computes_to_econstructor.
-    pose proof transform_id_left as H'; simpl in H'; rewrite H'.
-    reflexivity.
-    unfold ethernet_Frame_OK; unfold GetAttribute, GetAttributeRaw; simpl; omega.
-    apply_compose.
-    eapply Enum_decode_correct.
-    admit.
-    solve_data_inv.
-    simpl; intros; exact I.
-    apply_compose.
-    intros; eapply decode_list_all_correct_ComposeOpt.
-    solve_data_inv.
-    simpl; intros.
-    computes_to_inv; injections.
-    pose proof transform_id_left as H'; simpl in H'; rewrite H'; reflexivity.
-    simpl; intros.
-    unfold encode_decode_correct_f; intuition eauto.
-    destruct data as [? [? [? [? [ ] ] ] ] ];
-      unfold GetAttribute, GetAttributeRaw in *;
-      simpl in *.
-    computes_to_inv; injections; subst; simpl.
-    unfold ethernet_Frame_OK, GetAttribute, GetAttributeRaw in H6; simpl in H6.
-    pose proof transform_id_left as H'; simpl in H'; rewrite H'.
-    instantiate (1 := fun p b' c => if (Compare_dec.lt_dec (|p|) 1501) then _ p b' c else None); cbv beta.
-    destruct (Compare_dec.lt_dec (|proj2|) 1501); intuition.
-    eexists env'; simpl; intuition eauto.
-    match goal with
-      |- ?f ?a ?b ?c = ?P =>
-      let P' := (eval pattern a, b, c in P) in
-      let f' := match P' with ?f a b c => f end in
-      try unify f f'; try reflexivity
-    end.
-    simpl in H7.
-    destruct (Compare_dec.lt_dec (|proj2|) 1501); try discriminate.
-    eexists _; eexists env;
-      intuition eauto; injections; eauto using idx_ibound_eq;
-        try match goal with
-              |-  ?data => destruct data;
-                             simpl in *; eauto
-            end.
-    admit.
-    admit.
-    intros; eauto.
-    intros; eauto.
-    apply Vector_predicate_rest_True.
-    intros; apply Vector_predicate_rest_True.
-    simpl; intros; exact I.
-    repeat (instantiate (1 := fun _ => True)).
-    unfold cache_inv_Property; intuition.
-    Grab Existential Variables.
-    exact (@weq _).
-    exact (@weq _).
-    exact (@weq _).
-    exact (@weq _).
-  Defined.
+  apply_compose.
+  eapply Nat_decode_correct.
+  intuition eauto using ethernet_Frame_OK_good_Len.
+  solve_data_inv.
+  apply_compose.
+  eapply Word_decode_correct.
+  solve_data_inv.
+  simpl; intros; exact I.
+  apply_compose.
+  eapply Word_decode_correct.
+  solve_data_inv.
+  simpl; intros; exact I.
+  apply_compose.
+  eapply Word_decode_correct.
+  solve_data_inv.
+  simpl; intros; exact I.
+  apply_compose.
+  eapply Word_decode_correct.
+  solve_data_inv.
+  simpl; intros; exact I.
+  apply_compose.
+  eapply Enum_decode_correct.
+  Discharge_NoDupVector.
+  solve_data_inv.
+  simpl; intros; exact I.
+  apply_compose.
+  intros; eapply decode_list_all_correct_ComposeOpt.
+  solve_data_inv.
+  simpl; intros.
+  computes_to_inv; injections.
+  pose proof transform_id_left as H'; simpl in H'; rewrite H'; reflexivity.
+  simpl; intros.
+  unfold encode_decode_correct_f; intuition eauto.
+  unfold ethernet_Frame_OK in *.
+  instantiate (1 := fun p b' c => if (DecideableEnsembles.A_eq_dec (|p|) proj1) then
+                                    _ p b' c
+                                  else None).
+  instantiate (1 := fun p b' c =>
+                      if Compare_dec.lt_dec proj1 1501 then _ p b' c else None).
+  simpl.
+  destruct (Peano_dec.eq_nat_dec (|proj3|) proj1); try congruence.
+  destruct (Compare_dec.lt_dec proj1 1501); try congruence.
+  destruct data as [? [? [? [? [ ] ] ] ] ];
+    unfold GetAttribute, GetAttributeRaw in *;
+    simpl in *.
+  unfold ethernet_Frame_OK, GetAttribute, GetAttributeRaw in H15.
+  simpl in H15.
+  computes_to_inv; injections; subst; simpl.
+  pose proof transform_id_left as H'; simpl in H'; rewrite H'.
+  eexists env'; simpl; intuition eauto.
+  match goal with
+    |- ?f ?a ?b ?c = ?P =>
+    let P' := (eval pattern a, b, c in P) in
+    let f' := match P' with ?f a b c => f end in
+    try unify f f'; try reflexivity
+  end.
+  rewrite <- H17 in n; destruct n; eauto.
+  rewrite <- H15, <- H17 in n;
+  destruct n; reflexivity.
+  simpl in H12; repeat find_if_inside; try discriminate.
+  eexists _; eexists tt;
+    intuition eauto; injections; eauto using idx_ibound_eq;
+      try match goal with
+            |-  ?data => destruct data;
+                           simpl in *; eauto
+          end.
+  destruct env; computes_to_econstructor.
+  pose proof transform_id_left as H'; simpl in H'; rewrite H'.
+  reflexivity.
+  apply_compose.
+  eapply Enum_decode_correct.
+  Discharge_NoDupVector.
+  solve_data_inv.
+  simpl; intros; exact I.
+  apply_compose.
+  intros; eapply decode_list_all_correct_ComposeOpt.
+  solve_data_inv.
+  simpl; intros.
+  computes_to_inv; injections.
+  pose proof transform_id_left as H'; simpl in H'; rewrite H'; reflexivity.
+  simpl; intros.
+  unfold encode_decode_correct_f; intuition eauto.
+  unfold ethernet_Frame_OK in *.
+  instantiate (1 := fun p b' c =>
+                      if Compare_dec.lt_dec (|p|) 1501 then _ p b' c else None).
+  simpl.
+  destruct (Compare_dec.lt_dec (|proj2 |) 1501); try congruence.
+  destruct data as [? [? [? [? [ ] ] ] ] ];
+    unfold GetAttribute, GetAttributeRaw in *;
+    simpl in *.
+  computes_to_inv; injections; subst; simpl.
+  pose proof transform_id_left as H'; simpl in H'; rewrite H'.
+  eexists env'; simpl; intuition eauto.
+  match goal with
+    |- ?f ?a ?b ?c = ?P =>
+    let P' := (eval pattern a, b, c in P) in
+    let f' := match P' with ?f a b c => f end in
+    try unify f f'; try reflexivity
+  end.
+  rewrite <- H10 in n; destruct n; eauto.
+  simpl in *; repeat find_if_inside; try discriminate.
+  eexists _; eexists tt;
+    intuition eauto; injections; eauto using idx_ibound_eq;
+      try match goal with
+            |-  ?data => destruct data;
+                           simpl in *; eauto
+          end.
+  destruct env; computes_to_econstructor.
+  pose proof transform_id_left as H'; simpl in H'; rewrite H'.
+  reflexivity.
+  intros; eapply v1042_OKT; intuition eauto.
+  intros; eapply v1042_OKE; intuition eauto.
+  repeat (instantiate (1 := fun _ => True)).
+  unfold cache_inv_Property; intuition.
+  Grab Existential Variables.
+  exact (@weq _).
+  exact (@weq _).
+  exact (@weq _).
+  exact (@weq _).
+Defined.
 
-  Definition frame_decoder := Eval simpl in projT1 packet_decoder.
-  Print frame_decoder.
+Definition frame_decoder := Eval simpl in projT1 EthernetFrame_decoder.
+Print frame_decoder.
